
\documentclass{article}
\usepackage{amsmath}

%%%%%%%%%%%%%%%%%%%%%%%%%%%%%%%%%%%%%%%%%%%%%%%%%%%%%%%%%%%%%%%%%%%%%%%%%%%%%%%%%%%%%%%%%%%%%%%%%%%%%%%%%%%%%%%%%%%%%%%%%%%%%%%%%%%%%%%%%%%%%%%%%%%%%%%%%%%%%%%%%%%%%%%%%%%%%%%%%%%%%%%%%%%%%%%%%%%%%%%%%%%%%%%%%%%%%%%%%%%%%%%%%%%%
%TCIDATA{OutputFilter=LATEX.DLL}
%TCIDATA{Version=5.00.0.2552}
%TCIDATA{<META NAME="SaveForMode" CONTENT="1">}
%TCIDATA{Created=Saturday, October 03, 2015 15:22:22}
%TCIDATA{LastRevised=Saturday, October 03, 2015 20:08:49}
%TCIDATA{<META NAME="GraphicsSave" CONTENT="32">}
%TCIDATA{<META NAME="DocumentShell" CONTENT="Standard LaTeX\Blank - Standard LaTeX Article">}
%TCIDATA{CSTFile=40 LaTeX article.cst}

\newtheorem{theorem}{Theorem}
\newtheorem{acknowledgement}[theorem]{Acknowledgement}
\newtheorem{algorithm}[theorem]{Algorithm}
\newtheorem{axiom}[theorem]{Axiom}
\newtheorem{case}[theorem]{Case}
\newtheorem{claim}[theorem]{Claim}
\newtheorem{conclusion}[theorem]{Conclusion}
\newtheorem{condition}[theorem]{Condition}
\newtheorem{conjecture}[theorem]{Conjecture}
\newtheorem{corollary}[theorem]{Corollary}
\newtheorem{criterion}[theorem]{Criterion}
\newtheorem{definition}[theorem]{Definition}
\newtheorem{example}[theorem]{Example}
\newtheorem{exercise}[theorem]{Exercise}
\newtheorem{lemma}[theorem]{Lemma}
\newtheorem{notation}[theorem]{Notation}
\newtheorem{problem}[theorem]{Problem}
\newtheorem{proposition}[theorem]{Proposition}
\newtheorem{remark}[theorem]{Remark}
\newtheorem{solution}[theorem]{Solution}
\newtheorem{summary}[theorem]{Summary}
\newenvironment{proof}[1][Proof]{\noindent\textbf{#1.} }{\ \rule{0.5em}{0.5em}}


\begin{document}


$S^{2}=\frac{1}{n-1}\overset{n}{\underset{i=1}{\sum }}\left( X_{i}-\overline{%
X}\right) ^{2}.$

$\bigskip \mu _{4}=E\left( X_{1}-\mu \right) ^{4};\left( \text{4th central
moment of }X_{1}\right) $

$E\left( S^{4}\right) =\frac{1}{\left( n-1\right) ^{2}}E\left[ \overset{n}{%
\underset{i=1}{\sum }}\left( \left( X_{i}-\mu \right) -\left( \overline{X}%
-\mu \right) \right) ^{2}\right] ^{2}$

$E\left[ \overset{n}{\underset{i=1}{\sum }}\left( \left( X_{i}-\mu \right)
-\left( \overline{X}-\mu \right) \right) ^{2}\right] ^{2}=E\left[ \overset{n}%
{\underset{i=1}{\sum }}\left( X_{i}-\mu \right) ^{2}+n\left( \overline{X}%
-\mu \right) ^{2}-2\left( \overset{n}{\underset{i=1}{\sum }}\left( X_{i}-\mu
\right) \right) \left( \overline{X}-\mu \right) \right] ^{2}$

=$E\left[ \overset{n}{\underset{i=1}{\sum }}\left( X_{i}-\mu \right)
^{2}-n\left( \overline{X}-\mu \right) ^{2}\right] ^{2}$

=$E\left[ \overset{n}{\underset{i=1}{\sum }}\left( X_{i}-\mu \right) ^{2}%
\right] ^{2}+n^{2}E\left( \overline{X}-\mu \right) ^{4}-2n\overset{n}{%
\underset{i=1}{\sum }}E\left[ \left( X_{i}-\mu \right) ^{2}\left( \overline{X%
}-\mu \right) ^{2}\right] $

$=n\mu _{4}+\left( n^{2}-n\right) \sigma ^{4}+\frac{E\left[ \overset{n}{%
\underset{i=1}{\sum }}\left( X_{i}-\mu \right) \right] ^{4}}{n^{2}}-2n^{2}E%
\left[ \left( X_{1}-\mu \right) ^{2}\left( \overline{X}-\mu \right) ^{2}%
\right] $

=$n\mu _{4}+\left( n^{2}-n\right) \sigma ^{4}+\frac{n\mu _{4}+3n\left(
n-1\right) \sigma ^{4}}{n^{2}}-2E\left[ \left( X_{1}-\mu \right) ^{2}\overset%
{n}{\underset{i=1}{\sum }}\left( X_{i}-\mu \right) \right] $

=$n\mu _{4}+\left( n^{2}-n\right) \sigma ^{4}+\frac{n\mu _{4}+3n\left(
n-1\right) \sigma ^{4}}{n^{2}}-2\left[ \mu _{4}+\left( n-1\right) \sigma ^{4}%
\right] $

Then $D(S^{2})=E\left( S^{4}\right) -E^{2}\left( S^{2}\right) $

=$\frac{1}{\left( n-1\right) ^{2}}\left[ n\mu _{4}+\left( n^{2}-n\right)
\sigma ^{4}+\frac{n\mu _{4}+3n\left( n-1\right) \sigma ^{4}}{n^{2}}-2\left(
\mu _{4}+\left( n-1\right) \sigma ^{4}\right) \right] -\sigma ^{4}$

$=\frac{\mu _{4}-\sigma ^{4}}{n}+\frac{2\sigma ^{4}}{n\left( n-1\right) }$.

$\bigskip $

\end{document}
